SV_float.v
@@ -1,0 +1,759 @@
+Set Implicit Arguments.
+From SLF Require Import LabType Fun LibSepFmap Sum Unary_IndexWithBounds.
+From SLF Require Import LibWP LibSepSimpl LibSepReference LibSepTLCbuffer Struct Struct2 Loops Loops2 Loops_float ListCommon.
+From mathcomp Require Import ssreflect ssrfun zify.
+Hint Rewrite conseq_cons' : rew_listx.
+
+From Coq Require Import Permutation.
+
+Open Scope Z_scope.
+
+(* TODO maybe move this somewhere else *)
+Module incr_float.
+
+Section incr_float. 
+
+Context {D : Type}.
+
+Definition func :=
+  (<{ fun "real_j" "x" =>
+      let "tmp1" = ! "real_j" in
+      let "tmp2" = "tmp1" .+ "x" in
+      "real_j" := "tmp2" }>).
+
+Lemma spec `{Inhab D} (pj0 : loc) (d : D) (j x : binary64) :
+  htriple (single d tt)
+  (fun=> func pj0 x) 
+  (pj0 ~(d)~> val_float j)
+    (fun=> pj0 ~(d)~> val_float (j + x)%F64).
+Proof. by do 3 (xwp; xapp). Qed.
+
+End incr_float.
+End incr_float.
+
+Notation "k '.+=' x" :=
+  (incr_float.func k x)
+  (in custom trm at level 58, format "k  .+=  x") : trm_scope.
+
+Definition to_float (v : val) : binary64 := 
+  match v with 
+  | val_float i => i 
+  | _ => float_unit
+  end.
+
+Coercion to_float : val >-> binary64.
+
+Lemma to_float_if P a b : 
+  to_float (If P then a else b) = If P then a else b.
+Proof. by case: classicT. Qed.
+
+Module sv.
+
+Notation "H1 '\\*' H2" := (hstar H1 H2)
+  (at level 42, right associativity, format "H1  \\* '//' H2") : hprop_scope.
+
+Section sv.
+
+Notation "'xind'" := ("x_ind":var) (in custom trm at level 0) : trm_scope.
+Notation "'xval'" := ("x_val":var) (in custom trm at level 0) : trm_scope.
+Notation "'dvec'" := ("d_vec":var) (in custom trm at level 0) : trm_scope.
+(* sometimes Coq cannot tell whether lb is a variable or an int, so avoid using the same name lb here *)
+Notation "'xlb'" := ("l_b":var) (in custom trm at level 0) : trm_scope.
+Notation "'xrb'" := ("r_b":var) (in custom trm at level 0) : trm_scope.
+
+Import List Vars.
+
+(* TODO maybe move these somewhere else *)
+Section pure_facts.
+
+Fact fold_left_BPLUS_unit n : fold_left (@BPLUS _ Tdouble) (repeat float_unit n) float_unit = float_unit.
+Proof. induction n; auto. Qed.
+
+Variable (M : int) (l : list int).
+Hypothesis (HM : 0 <= M) (* avoid the case where l is nil and M can be anything *). 
+Hypotheses (Hnodup : NoDup l) (Hbounded : forall x, In x l -> 0 <= x < M).
+
+Fact nodup_bounded_saturate : length l = M :> int -> Permutation (lof id M) l.
+Admitted.
+
+Fact nodup_bounded_saturate' : length l = M :> int -> forall x : int, 0 <= x < M -> In x l.
+Admitted.
+
+Fact nodup_bounded_makeperm_bysuf : exists l' : list int, 
+  NoDup (List.app l l') /\ (forall x, In x (List.app l l') -> 0 <= x < M) /\ (length (List.app l l') = M :> int).
+Admitted.
+
+Fact nodup_bounded_makeperm_bypre : exists l' : list int, 
+  NoDup (List.app l' l) /\ (forall x, In x (List.app l' l) -> 0 <= x < M) /\ (length (List.app l' l) = M :> int).
+Admitted.
+
+Fact nodup_bounded_length_le : length l <= M.
+Proof.
+  (*
+  destruct (Z.leb (Z.of_nat (length l)) M) eqn:E.
+  1: apply Z.leb_le in E; math.
+  apply Z.leb_gt in E. destruct l as [ | x l' ]; clear l; simpl in E; try math.
+  assert (M <= length l') as Hle by math.
+  inversion_clear Hnodup. false H.
+  simpl in Hbounded. 
+  *)
+Admitted.
+
+End pure_facts.
+
+Context (xind : list int).
+Context (xval : list binary64).
+Context (N M : int).
+Context (lb rb : int).
+Hypothesis (len : rb - lb = N).
+Hypotheses (bounds_l: 0 <= lb) (bounds_r: lb <= rb).
+Hypothesis len_xind : rb <= length xind.
+Hypothesis len_xval : rb <= length xval.
+Hypothesis nodup_xind : NoDup (list_interval (abs lb) (abs rb) xind).
+Hypothesis xind_leq : forall x, In x (list_interval (abs lb) (abs rb) xind) -> 0 <= x < M.
+
+Definition indexf := index_bounded.func.
+
+Definition get := 
+  <{
+  fun i xind xval xlb xrb =>
+    let k = indexf xlb xrb i xind in 
+    let "k < rb" = k < xrb in
+    if "k < rb" then
+      xval[.k]
+    else float_unit
+}>.
+
+Lemma get_spec {D} `{Inhab D} (x_ind x_val : loc) d (l : int): 
+  @htriple D (single d tt) 
+    (fun=> get l x_ind x_val lb rb)
+    (harray_int xind x_ind d \* 
+      harray_float xval x_val d)
+    (fun hr => 
+      harray_int xind x_ind d \* 
+      harray_float xval x_val d).
+Proof.
+  rewrite -wp_equiv; xsimpl.
+  xwp; xapp @index_bounded.spec=> //.
+  xwp; xapp; xwp; xif=> ?; [xapp|xwp;xval]; xsimpl.
+Qed.
+
+Lemma get_spec_in {D : Type} `{Inhab D} (x_ind x_val : loc) i d : 
+  @htriple D (single d tt) 
+    (fun=> get (List.nth (abs i) (list_interval (abs lb) (abs rb) xind) 0) x_ind x_val lb rb)
+    (\[0 <= i < N] \*
+      harray_int xind x_ind d \* 
+      harray_float xval x_val d)
+    (fun hr => 
+     \[hr = fun=> List.nth (abs i) (list_interval (abs lb) (abs rb) xval) 0] \* 
+      harray_int xind x_ind d \* 
+      harray_float xval x_val d).
+Proof.
+  rewrite -wp_equiv; xsimpl=> ?.
+  xwp; xapp (@index_bounded.spec _ H)=> //.
+  xwp; xapp.
+  rewrite index_nodup; auto.
+  2: rewrite list_interval_length; subst; auto.
+  xwp; xif=> ?; subst; try math.
+  xapp; xsimpl*. rewrite -> list_interval_nth with (rb:=rb); try math; auto.
+Qed.
+
+Lemma get_spec_out_unary {D : Type} `{Inhab D} (x_ind x_val : loc) (i : int) d : 
+  @htriple D (single d tt) 
+    (fun=> get i x_ind x_val lb rb)
+    (\[~ In i (list_interval (abs lb) (abs rb) xind)] \*
+      harray_int xind x_ind d \* 
+      harray_float xval x_val d)
+    (fun hr => 
+     \[hr = fun=> float_unit] \* 
+      harray_int xind x_ind d \* 
+      harray_float xval x_val d).
+Proof.
+  rewrite -wp_equiv; xsimpl=> ?.
+  xwp; xapp (@index_bounded.spec _ H)=> //...
+  rewrite memNindex // list_interval_length //.
+  xwp; xapp. xwp; xif=> ?; try math. xwp; xval. xsimpl*.
+Qed.
+
+Local Notation D := (labeled int).
+
+Lemma get_spec_out `{Inhab D} fs (x_ind x_val : loc) : 
+  @htriple D fs
+    (fun i => get (eld i) x_ind x_val lb rb)
+    (\[forall d, indom fs d -> ~ In (eld d) (list_interval (abs lb) (abs rb) xind)] \*
+      (\*_(d <- fs) harray_int xind x_ind d) \* 
+       \*_(d <- fs) harray_float xval x_val d)
+    (fun hr => 
+     \[hr = fun=> float_unit] \* 
+      ((\*_(d <- fs) harray_int xind x_ind d) \* 
+       \*_(d <- fs) harray_float xval x_val d)).
+Proof.
+  apply/htriple_val_eq/htriple_conseq;
+  [|eauto|move=> ?]; rewrite -hstar_fset_pure -?hbig_fset_hstar; first last.
+  { move=> ?; apply: applys_eq_init; reflexivity. }
+  apply/htriple_union_pointwise=> [> -> //|??]. 
+  rewrite -wp_equiv wp_single; xapp (@get_spec_out_unary D)=> // ??->.
+  xsimpl*.
+Qed.
+
+Definition sum := 
+  <{
+  fun xind xval xlb xrb =>
+  let s = ref float_unit in
+  for i <- [xlb, xrb] {
+    let x = xval[.i] in 
+    (* s += x *)
+    s .+= x
+  };
+  let "res" = ! s in
+  free s;
+  "res"
+}>.
+
+(* Tactic Notation "xin" constr(S1) ":" tactic(tac) := 
+  let n := constr:(S1) in
+  xfocus n; tac; try(
+  first [xunfocus | xcleanup n]; simpl; try apply xnwp0_lemma). *)
+Lemma val_float_eq i j : 
+  (val_float i = val_float j) = (i = j).
+Proof. by extens; split=> [[]|]->. Qed.
+
+Ltac fold' := 
+  rewrite ?label_single ?wp_single ?val_float_eq
+    (* -/(incr _)  *)
+    -/float_unit
+    -/(For_aux _ _) 
+    -/(For _ _ _) //=.
+
+Fact Union_interval_change2 [A : Type] (f : int -> fset A) (a b : int) :
+  Union (interval 0 (b - a)) f = Union (interval a b) (fun i => f (i - a)).
+Proof. 
+  rewrite -> Union_interval_change with (c := a).
+  do ? f_equal; lia.
+Qed.
+(*
+Fact Sum_interval_change2 (f : int -> int) (a b : int) :
+  Sum (interval 0 (b - a)) f = Sum (interval a b) (fun i => f (i - a)).
+Proof.
+  rewrite -> Sum_interval_change with (c := a).
+  do ? f_equal; lia.
+Qed.
+
+Fact Sum1 {A : Type} (s : A) (f : A -> int) : 
+  Sum (`{s}) f = f s.
+Proof.
+  rewrite update_empty SumUpdate; [ rewrite Sum0 Z.add_0_l; reflexivity | auto ].
+Qed.
+*)
+Lemma lhtriple_free : forall (p : loc) (v : val) fs,
+  @htriple D fs (fun d => val_free p)
+    (\*_(d <- fs) p ~(d)~> v)
+    (fun _ => \[]).
+Proof using. intros. apply htriple_free. Qed.
+
+Hint Resolve lhtriple_free : lhtriple.
+
+Notation "l '[[' i '--' j ']]' " := (list_interval (abs i) (abs j) l) (at level 5).
+
+Lemma sum_spec `{Inhab D} (x_ind x_val : loc) : 
+  {{ arr(x_ind, xind)⟨1, 0⟩ \*
+     .arr(x_val, xval)⟨1, 0⟩ \\* 
+     (\*_(i <- `[0, M]) arr(x_ind, xind)⟨2, i⟩) \\*
+     (\*_(i <- `[0, M]) .arr(x_val, xval)⟨2, i⟩) }}
+  [{
+    [1| ld in `{0}         => sum x_ind x_val lb rb];
+    {2| ld in `[0, M]          => get ld x_ind x_val lb rb}
+  }]
+  {{ hv, (\exists perm : list int, 
+    \[Permutation (lof id M) perm /\ 
+    (* stating that xind is a subsequence of perm may be beneficial, but is it needed? *)
+    (* this is exact, no feq is needed *)
+    (hv[`1](0)) = val_float (fold_left (@BPLUS _ Tdouble) 
+    (projT1 (@list_of_fun' _ float_unit (fun i => to_float (hv[`2](perm[i]))) M)) float_unit)]) \* 
+      arr(x_ind, xind)⟨1, 0⟩ \*
+      .arr(x_val, xval)⟨1, 0⟩ \* 
+      (\*_(i <- `[0, M]) arr(x_ind, xind)⟨2, i⟩) \\*
+      (\*_(i <- `[0, M]) .arr(x_val, xval)⟨2, i⟩)}}.
+Proof with fold'.
+  xfocus (2,0) xind[[lb -- rb]].
+  rewrite (hbig_fset_part (`[0, M]) xind[[lb -- rb]]). (* TODO: move to xfocus *)
+  xapp get_spec_out=> //.
+  { case=> ?? /[! @indom_label_eq]-[_]/=; rewrite /intr filter_indom; autos*. }
+  set (H1 := hbig_fset hstar (_ ∖ _) _); set (H2 := hbig_fset hstar (_ ∖ _) _).
+  xframe2 H1. xframe2 H2. xsimpl.
+  xin (1,0) : xwp; xapp=> q...
+  have Hl : length xind[[lb -- rb]] = rb - lb :> int.
+  1: rewrite -> list_interval_length; try math.
+  rewrite intr_list ?(fset_of_list_nodup 0) ?Hl ?Union_interval_change2 //.
+  set (R (i : int) := arr(x_ind, xind)⟨2, i⟩ \* .arr(x_val, xval)⟨2, i⟩).
+  set (Inv (i : int) := arr(x_ind, xind)⟨1, 0⟩ \* .arr(x_val, xval)⟨1, 0⟩).
+  xfor_sum_float Inv R R (fun hv i => hv[`2](xind[i])) q.
+  { rewrite /Inv /R.
+    (xin (1,0): (xwp; xapp; xapp (@incr_float.spec  _ H)=> y))...
+    xapp (@get_spec_in D)=> //; try math. xsimpl*.
+    rewrite <- list_interval_nth with (l:=xval); try math.
+    replace (lb + (l0 - lb)) with l0 by math. xsimpl*. }
+  { intros Hneq Hi Hj Hq. apply Hneq. 
+    enough (abs (i0 - lb) = abs (j0 - lb) :> nat) by math.
+    eapply NoDup_nth. 4: apply Hq. all: try math; try assumption. }  
+  { rewrite -list_interval_nth; try f_equal; lia. }
+  xwp; xapp... xwp; xapp. xwp; xval. 
+  case (classicT (0 <= M))=> C.
+  2: admit.
+  (* long and hard, but still possible to be extracted and solved *)
+  pose proof (nodup_bounded_makeperm_bypre C nodup_xind xind_leq) as (l' & Hnodup & Hbounded & Hlen).
+  xsimpl* (List.app l' (xind [[lb -- rb]])). 
+  split. 1: by apply nodup_bounded_saturate.
+  pose proof (nodup_bounded_length_le C nodup_xind xind_leq) as Hle.
+  rewrite list_interval_length in Hle...
+  destruct (list_of_fun' _ _) as (l1 & Hlen1 & Hl1); simpl.
+  destruct (list_of_fun' _ _) as (l2 & Hlen2 & Hl2); simpl.
+  assert (l2 = (repeat float_unit (abs (M - N))) ++ l1) as ->.
+  { apply List.nth_ext with (d:=float_unit) (d':=float_unit).
+    1: rewrite List.app_length repeat_length; math.
+    intros i0 Hi0. replace i0 with (abs i0) by math.
+    rewrite -> Hl2; try math. case_if.
+    { rewrite /Sum.mem in C0.
+      admit. } 
+    { admit. } }
+  rewrite fold_left_app fold_left_BPLUS_unit //.
+Abort.
+(*
+Context (dvec : list int).
+Context (dvec_len : length dvec = M :> int).
+
+Definition dotprod := 
+  <{
+  fun xind xval dvec xlb xrb =>
+  let s = ref 0 in
+  for i <- [xlb, xrb] {
+    let x = xval[i] in 
+    let i = xind[i] in 
+    let v = dvec[i] in 
+    let x = x * v in
+    s += x
+  };
+  let "res" = ! s in
+  free s;
+  "res"
+}>.
+
+Lemma SumIf {A : Type} {P : A -> Prop} {fs F G} (C : A -> int -> int) : 
+  (Σ_(i <- fs) C i (If P i then F i else G i)) = 
+  Σ_(i <- fs ∩ P) C i (F i) + Σ_(i <- fs ∖ P) C i (G i).
+Proof using.
+Admitted.
+
+Lemma dotprod_spec `{Inhab D} (x_ind x_val d_vec : loc) : 
+  {{ arr(x_ind, xind)⟨1, 0⟩ \\*
+     arr(x_val, xval)⟨1, 0⟩ \\*
+     arr(d_vec, dvec)⟨1, 0⟩ \\* 
+     (\*_(i <- `[0, M]) arr(x_ind, xind)⟨2, i⟩) \\*
+     (\*_(i <- `[0, M]) arr(x_val, xval)⟨2, i⟩) \\* 
+     (\*_(i <- `[0, M]) arr(d_vec, dvec)⟨2, i⟩) }}
+  [{
+    [1| ld in `{0}   => dotprod x_ind x_val d_vec lb rb];
+    [2| ld in `[0,M] => get ld x_ind x_val lb rb]
+  }]
+  {{ hv, \[hv[`1](0) = Σ_(i <- `[0,M]) (hv[`2](i) * dvec[i])] \* 
+     arr(x_ind, xind)⟨1, 0⟩ \\*
+     arr(x_val, xval)⟨1, 0⟩ \\*
+     arr(d_vec, dvec)⟨1, 0⟩ \\* 
+     (\*_(i <- `[0, M]) arr(x_ind, xind)⟨2, i⟩) \\*
+     (\*_(i <- `[0, M]) arr(x_val, xval)⟨2, i⟩) \\* 
+     (\*_(i <- `[0, M]) arr(d_vec, dvec)⟨2, i⟩)}}.
+Proof with fold'.
+  xfocus (2,0) xind[[lb -- rb]].
+  rewrite (hbig_fset_part (`[0, M]) xind[[lb -- rb]]). (* TODO: move to xfocus *)
+  xapp get_spec_out=> //.
+  { case=> ?? /[! @indom_label_eq]-[_]/=; rewrite /intr filter_indom; autos*. }
+  repeat let HH := fresh "uselessheap" in set (HH := hbig_fset hstar (_ ∖ _) _); xframe2 HH; xsimpl.
+  xin (1,0) : xwp; xapp=> q...
+  have Hl : length xind[[lb -- rb]] = rb - lb :> int.
+  1: rewrite -> list_interval_length; try math.
+  rewrite intr_list ?(fset_of_list_nodup 0) ?Hl ?Union_interval_change2 //.
+  set (R (i : int) := arr(x_ind, xind)⟨2, i⟩ \* arr(x_val, xval)⟨2, i⟩ \* arr(d_vec, dvec)⟨2,i⟩).
+  set (Inv (i : int) := arr(x_ind, xind)⟨1, 0⟩ \* arr(x_val, xval)⟨1, 0⟩ \* arr(d_vec, dvec)⟨1,0⟩).
+  xfor_sum Inv R R (fun hv i => (hv[`2](xind[i]) * dvec[xind[i] ])) q.
+  { rewrite /Inv /R.
+    (xin (1,0): do 4 (xwp; xapp); xapp (@incr.spec _ H)=> y)...
+    xapp (@get_spec_in D)=> //; try math. xsimpl*.
+    rewrite <- list_interval_nth with (l:=xval); try math.
+    replace (lb + (l0 - lb)) with l0 by math. xsimpl*. }
+  { intros Hneq Hi Hj Hq. apply Hneq. 
+    enough (abs (i0 - lb) = abs (j0 - lb) :> nat) by math.
+    eapply NoDup_nth. 4: apply Hq. all: try math; try assumption. }
+  { rewrite -list_interval_nth; try f_equal; lia. }
+  xwp; xapp... xwp; xapp. xwp; xval. xsimpl*.
+  f_equal; under (@SumEq _ _ _ (`[0, M])).
+  { move=>*; rewrite to_int_if; over. }
+  rewrite (SumIf (fun=> Z.mul^~ _)) intr_list // Sum0s Sum_list_interval //; math.
+Qed.
+*)
+End sv. 
+(*
+Section sv.
+
+Import List.
+
+Definition slice {A} (l : list A) i j := (list_interval (abs i) (abs j) l).
+
+Context (xind xval yind yval : list int).
+Context (Nx Ny M rbx lbx rby lby : int).
+(* Hypothesis lenx : rbx - lbx = Nx. *)
+(* Hypothesis leny : rby - lby = Nx. *)
+Hypothesis (bounds_lx : 0 <= lbx) (bound_rx : lbx <= rbx).
+Hypothesis (bounds_ly : 0 <= lby) (bound_ry : lby <= rby).
+Hypothesis len_xind : rbx <= length xind.
+Hypothesis len_xval : rbx <= length xval.
+Hypothesis len_yind : rby <= length yind.
+Hypothesis len_yval : rby <= length yval.
+Hypothesis sorted_xind : sorted (slice xind lbx rbx).
+Hypothesis sorted_yind : sorted (slice yind lby rby).
+Hypothesis xind_leq : forall x, In x (slice xind lbx rbx) -> 0 <= x < M.
+Hypothesis yind_leq : forall x, In x (slice yind lby rby) -> 0 <= x < M.
+
+
+(* Notation "'xind'" := ("x_ind":var) (in custom trm at level 0) : trm_scope. *)
+(* Notation "'xval'" := ("x_val":var) (in custom trm at level 0) : trm_scope. *)
+(* Notation "'yind'" := ("y_ind":var) (in custom trm at level 0) : trm_scope. *)
+(* Notation "'yval'" := ("y_val":var) (in custom trm at level 0) : trm_scope. *)
+Notation "'rbx'" := ("rb_x":var) (in custom trm at level 0) : trm_scope.
+Notation "'lbx'" := ("lb_x":var) (in custom trm at level 0) : trm_scope.
+Notation "'rby'" := ("rb_y":var) (in custom trm at level 0) : trm_scope.
+Notation "'lby'" := ("lb_y":var) (in custom trm at level 0) : trm_scope.
+Notation "'iX'" := ("iX":var) (in custom trm at level 0) : trm_scope.
+Notation "'iY'" := ("iY":var) (in custom trm at level 0) : trm_scope.
+Notation "'ans'" := ("ans":var) (in custom trm at level 0) : trm_scope.
+
+Notation "'while' C '{' T '}'"  :=
+  (While C T)
+  (in custom trm at level 69,
+    C, T at level 0,
+    format "'[' while  C ']'  '{' '/   ' '[' T  '}' ']'") : trm_scope.
+
+Definition sv_dotprod (xind yind xval yval : loc) := <{
+  fun lbx rbx lby rby  =>
+    let ans = ref 0 in
+    let iX = ref lbx in 
+    let iY = ref lby in 
+      while (
+        let "ix" = !iX in
+        let "iy" = !iY in
+        let "iXl" = "ix" < rbx in 
+        let "iYl" = "iy" < rby in
+        "iXl" && "iYl") {
+        let "ix" = !iX in
+        let "iy" = !iY in
+        let "iXind" = xind["ix"] in 
+        let "iYind" = yind["iy"] in 
+        let "cnd" = "iXind" = "iYind" in 
+        if "cnd" then 
+          let "iXind" = xval["ix"] in 
+          let "iYind" = yval["iy"] in 
+          let "val" = "iXind" * "iYind" in
+          ans += "val";
+          ++iX;
+          ++iY
+        else 
+          let "cnd" = "iXind" < "iYind" in 
+          if "cnd" then 
+            ++iX 
+          else ++iY
+      }; 
+      let "s" = !ans in 
+      free iX; free iY; free ans;
+      "s"
+}>.
+
+Definition arr1 x_ind y_ind x_val y_val := 
+  arr(x_ind, xind)⟨1, 0⟩ \* arr(y_ind, yind)⟨1, 0⟩ \*
+  arr(x_val, xval)⟨1, 0⟩ \* arr(y_val, yval)⟨1, 0⟩.
+
+Ltac fold' := 
+  rewrite ?label_single ?wp_single ?val_int_eq
+    -/(While_aux _ _) 
+    -/(While _ _) //=; try lia.
+
+Notation size := Datatypes.length.
+
+Lemma not_isTrueE (P: Prop) : (~ isTrue P) = ~ P.
+Proof.
+Admitted.
+
+Ltac bool_rew := 
+  rewrite ?false_eq_isTrue_eq ?istrue_isTrue_eq 
+    ?true_eq_isTrue_eq -?(isTrue_and, isTrue_not, isTrue_or) ?not_isTrueE.
+
+Hint Resolve lhtriple_free : lhtriple.
+
+Lemma sv_dotprod_spec `{Inhab (labeled int)} (x_ind x_val y_ind y_val : loc) : 
+  {{ (arr(x_ind, xind)⟨1, 0⟩ \* arr(y_ind, yind)⟨1, 0⟩ \*
+     arr(x_val, xval)⟨1, 0⟩ \* arr(y_val, yval)⟨1, 0⟩) \*
+     (\*_(i <- `[0, M]) arr(x_ind, xind)⟨2, i⟩) \\*
+     (\*_(i <- `[0, M]) arr(x_val, xval)⟨2, i⟩) \\* 
+     (\*_(i <- `[0, M]) arr(y_ind, yind)⟨3, i⟩) \\*
+     (\*_(i <- `[0, M]) arr(y_val, yval)⟨3, i⟩) }}
+  [{
+    {1| ld in `{0}   => sv_dotprod x_ind y_ind x_val y_val lbx rbx lby rby};
+    {2| ld in `[0,M] => get ld x_ind x_val lbx rbx};
+    {3| ld in `[0,M] => get ld y_ind y_val lby rby}
+  }]
+  {{ hv, \[hv[`1](0) = Σ_(i <- `[0,M]) (hv[`2](i) * hv[`3](i))] \* 
+      (arr(x_ind, xind)⟨1, 0⟩ \* arr(y_ind, yind)⟨1, 0⟩ \*
+      arr(x_val, xval)⟨1, 0⟩ \* arr(y_val, yval)⟨1, 0⟩) \*
+      (\*_(i <- `[0, M]) arr(x_ind, xind)⟨2, i⟩) \\*
+      (\*_(i <- `[0, M]) arr(x_val, xval)⟨2, i⟩) \\* 
+      (\*_(i <- `[0, M]) arr(y_ind, yind)⟨3, i⟩) \\*
+      (\*_(i <- `[0, M]) arr(y_val, yval)⟨3, i⟩)}}.
+Proof with fold'.
+  set (sxind := (slice xind lbx rbx)).
+  set (syind := (slice yind lby rby)).
+  set (sxval := (slice xval lbx rbx)).
+  set (syval := (slice yval lby rby)).
+  set (ind := merge sxind syind).
+  have?: NoDup sxind by exact/sorted_nodup.
+  have?: NoDup syind by exact/sorted_nodup.
+  rewrite -/(arr1 _ _ _ _).
+  have ndind: NoDup ind by exact/sorted_nodup/sorted_merge.
+  xfocus (2,0) (ind).
+  rewrite {1 2 5 6}(hbig_fset_part `[0, M] ind).
+  xapp (@get_spec_out xind xval); eauto.
+  { case=> ??/=/[!@indom_label_eq]-[_].
+    rewrite /intr filter_indom/= /Sum.mem/ind In_merge; autos*. }
+  set (H1 := hbig_fset hstar (_ ∖ _) _); 
+  set (H2 := hbig_fset hstar (_ ∖ _) _).
+  xframe2 H1; xframe2 H2; xsimpl; clear H1 H2.
+  xfocus (3,0) ind.
+  rewrite (hbig_fset_part `[0, M] ind).
+  xapp (@get_spec_out yind yval); eauto.
+  { case=> ??/=/[!@indom_label_eq]-[_].
+    rewrite /intr filter_indom/= /Sum.mem/ind In_merge; autos*. }
+  set (H1 := hbig_fset hstar (_ ∖ _) _); 
+  set (H2 := hbig_fset hstar (_ ∖ _) _).
+  xframe2 H1; xframe2 H2; xsimpl; clear H1 H2.
+  set (H1 := _ \* hbig_fset _ _ _); set (H2 := _ \* H1); set (arrs := _ \* H2).
+  xin (1,0) : xwp; xapp=> ans; xwp; xapp=> iX; xwp; xapp=> iY...
+  have Hlx : length sxind = rbx - lbx :> int.
+  1: rewrite /sxind list_interval_length; try math.
+  have Hly : length syind = rby - lby :> int.
+  1: rewrite /syind list_interval_length; try math.
+  have E : `[0,M] ∩ ind = ind.
+  { apply/fset_extens=> ?. 
+    rewrite /intr filter_indom /ind -fset_of_list_in /Sum.mem ?In_merge; splits*.
+    rewrite ?indom_interval=> -[]; autos*. }
+  rewrite ?E (fset_of_list_nodup 0) //.
+  set (cond ix iy := isTrue (ix < rbx /\ iy < rby)).
+  set (Inv (b : bool) (i : int) := 
+    arr1 x_ind y_ind x_val y_val \*
+    \exists (ix iy : int), 
+      iY ~⟨(1, 0)%Z, 0⟩~> iy \* iX ~⟨(1, 0)%Z, 0⟩~> ix \*
+      \[(i = size ind -> ~ b) /\ lbx <= ix /\ lby <= iy /\
+        (i < size ind -> ind[i] > max (take (abs (ix - lbx)) sxind)) /\
+        (i < size ind -> ind[i] > max (take (abs (iy - lby)) syind)) /\ 
+        b = cond ix iy /\
+        (b -> 
+          (ind[i] = Z.min xind[ix] yind[iy] /\ 
+          (forall x, In x sxind -> x < xind[ix] -> x < yind[iy]) /\  
+          (forall y, In y syind -> y < yind[iy] -> y < xind[ix])))]).
+  set (op hv i := hv[`2](ind[i]) * hv[`3](ind[i])).
+  set (R1 (i : int) := arr(y_ind, yind)⟨3,i⟩ \* arr(y_val, yval)⟨3,i⟩).
+  set (R2 (i : int) := arr(x_ind, xind)⟨2,i⟩ \* arr(x_val, xval)⟨2,i⟩).
+  have xindE : forall i, lbx <= i < rbx -> xind[i] = sxind[i-lbx].
+  { move=> *; rewrite -list_interval_nth; try f_equal... }
+  have yindE : forall i, lby <= i < rby -> yind[i] = syind[i-lby].
+  { move=> *; rewrite -list_interval_nth; try f_equal... }
+  have xvalE : forall i, lbx <= i < rbx -> xval[i] = sxval[i-lbx].
+  { move=> *; rewrite -list_interval_nth; try f_equal... }
+  have yvalE : forall i, lby <= i < rby -> yval[i] = syval[i-lby].
+  { move=> *; rewrite -list_interval_nth; try f_equal... }
+  have sE : forall a b, a - b + 1 = a + 1 - b by lia.
+  xwhile_sum Inv R1 R2 R1 R2 op ans=> //.
+  { move=> l s ?.
+    rewrite {1}/Inv; xnsimpl=> ix iy[?][?][?][LM1][LM2][].
+    rewrite /cond. bool_rew=> -[??]/(_ eq_refl)-[]indlE[L1 L2].
+    rewrite /arr1; clear arrs H1 H2.
+    xin (1,0): do 5 (xwp; xapp); xwp; xif=> C.
+    { xin (1,0): 
+        do 3 (xwp; xapp); xwp; xapp @incr.spec; 
+        (xwp; xapp @incr1.spec); xapp @incr1.spec=> ?.
+      rewrite /op /=; rewrite <-?hstar_assoc.
+      set (Heap := _ \* harray_int xind _ _); rewrite /R2...
+      rewrite val_int_eq in C; rewrite {-1 4 6}indlE -C Z.min_id xindE...
+      xin (2,0): fold'; xapp get_spec_in; eauto...
+      rewrite /R1 indlE C Z.min_id yindE...
+      xapp get_spec_in; eauto...
+      rewrite /Heap /Inv /arr1/cond.
+      have SlE: 
+        l + 1 = size ind -> 
+          ~ (ix - lbx + 1 < rbx - lbx /\ iy - lby + 1 < rby - lby). 
+      { move: C indlE=>-> /[! Z.min_id]/[swap]/sorted_max_size->; bool_rew.
+        have: max ind >= max syind by apply/max_sublist=>?; rewrite In_merge; right.
+        rewrite yindE...
+        move=>/[swap]->/nth_le_max-> //; lia. }
+      rewrite -xvalE -?yvalE...
+      xsimpl (ix + 1) (iy + 1); splits; [|lia|lia| | |autos*|]...
+      { bool_rew... }
+      { move=> ?; rewrite -sE max_takeS -?xindE... 
+        suff: ind[l] < ind[l+1] by lia.
+        apply/sorted_le; autos*; try lia.
+        exact/sorted_merge. }
+      { replace (iy + 1 - lby) with (iy - lby + 1) by lia.
+        move=> ?; rewrite max_takeS -?yindE...
+        suff: ind[l] < ind[l+1] by lia.
+        apply/sorted_le; autos*; try lia.
+        exact/sorted_merge. }
+      bool_rew=> -[]??; splits*.
+      { rewrite merge_nthS // -/ind; try lia.
+        rewrite indlE {2}C -{1}C ?Z.min_id xindE ?yindE ?search_nth...
+        rewrite xindE ?yindE; first do 2 f_equal... }
+      { move=> x ??; move: (@sorted_le (iy -lby) (iy +1 - lby) syind sorted_yind).
+        rewrite -?yindE...
+        suff: (x <= xind[ix]) by lia.
+        rewrite xindE; first apply/In_lt; rewrite ?sE -?xindE... }
+      move=> y ??; move: (@sorted_le (ix -lbx) (ix +1 - lbx) sxind sorted_xind).
+      rewrite -?xindE...
+      suff: (y <= yind[iy]) by lia.
+      rewrite yindE; first apply/In_lt; rewrite ?sE -?yindE... }
+    rewrite /op.
+    xin (1,0): xwp; xapp; xwp; xif=> L; xapp @incr1.spec=> ?.
+    { rewrite /op /=; rewrite <-?hstar_assoc.
+      set (Heap := _ \* harray_int yval _ _); rewrite /R2...
+      rewrite indlE Z.min_l... rewrite (xindE ix)...
+      xin (2,0): fold'; xapp get_spec_in; eauto...
+      rewrite /R1; xapp get_spec_out_unary; eauto.
+      { move/L2; rewrite -xindE... }
+      rewrite Z.mul_0_r Z.add_0_r.
+      rewrite /Heap /Inv /arr1/cond.
+      have SlE: 
+        l + 1 = size ind -> 
+          ~ (ix - lbx + 1 < rbx - lbx /\ iy - lby < rby - lby). 
+      { move: indlE=> /[!Z.min_l] //; last lia. 
+        move=>/[swap]/sorted_max_size->; bool_rew.
+        have: max ind >= max sxind by apply/max_sublist=>?; rewrite In_merge; left.
+        move=>/[swap]->; rewrite xindE... move/nth_le_max->... }
+      xsimpl (ix + 1) (iy); splits; [|lia|lia| | |autos*|].
+      { bool_rew... }
+      { move=> ?; rewrite -sE max_takeS -?xindE...
+        suff: ind[l] < ind[l+1] by lia.
+        apply/sorted_le; autos*; try lia.
+        exact/sorted_merge. }
+      { move=> ?. suff: ind[l] < ind[l+1] by lia.
+        apply/sorted_le; autos*; try lia.
+        exact/sorted_merge. }
+      bool_rew=> -[]??; splits*.
+      { rewrite merge_nthS -/ind ?indlE 1?(Z.min_l (_[_]))...
+        rewrite xindE ?search_nth ?sE -?xindE ?yindE...
+        erewrite search_lt_nth; eauto...
+        all: rewrite -yindE...
+        move=> ? /L2; lia. }
+      { move=> x ??; move: (@sorted_le (ix -lbx) (ix +1 - lbx) sxind sorted_xind).
+        rewrite -?xindE...
+        suff: (x <= xind[ix]) by lia.
+        rewrite xindE; first apply/In_lt; rewrite ?sE -?xindE... }
+      move=> ? /L2/[apply]; rewrite ?xindE...
+      move:  (@sorted_le (ix -lbx) (ix +1 - lbx) sxind sorted_xind)... }
+    rewrite /op /=; rewrite <-?hstar_assoc.
+    set (Heap := _ \* harray_int yval _ _); rewrite /R1...
+    rewrite indlE Z.min_r... rewrite (yindE iy)...
+    xin (3,0): fold'; xapp get_spec_in...
+    rewrite /R2; xapp get_spec_out_unary; eauto.
+    { move/L1. rewrite val_int_eq in C; rewrite -yindE... }
+    rewrite Z.mul_0_l Z.add_0_r.
+    have SlE: 
+    l + 1 = size ind -> 
+      ~ (ix - lbx < rbx - lbx /\ iy - lby + 1 < rby - lby). 
+    { move: indlE=> /[!Z.min_r] //; last lia. 
+      move=>/[swap]/sorted_max_size->; bool_rew.
+      have: max ind >= max syind by apply/max_sublist=>?; rewrite In_merge; right.
+      move=>/[swap]->; rewrite yindE... move/nth_le_max->... }
+    rewrite val_int_eq in C.
+    rewrite /Heap /Inv /arr1/cond; xsimpl (ix) (iy+1); splits; [|lia|lia| | |autos*|].
+    { bool_rew... }
+    { move=> ?. suff: ind[l] < ind[l+1] by lia.
+      apply/sorted_le; autos*; try lia.
+      exact/sorted_merge. }
+    { move=> ?; rewrite -sE max_takeS -?yindE...
+      suff: ind[l] < ind[l+1] by lia.
+      apply/sorted_le; autos*; try lia.
+      exact/sorted_merge. }
+    bool_rew=> -[]??; splits*.
+    { rewrite merge_nthS -/ind ?indlE 1?(Z.min_r (_[_]))...
+      rewrite yindE ?search_nth ?sE -?yindE ?xindE...
+      erewrite search_lt_nth; eauto...
+      all: rewrite -xindE...
+      move=> ? /L1; lia. }
+    { move=> ? /L1/[apply]; rewrite ?yindE...
+      move: (@sorted_le (iy - lby) (iy+1-lby) syind sorted_yind); lia. }
+    move=> y ??; move: (@sorted_le (iy -lby) (iy +1 - lby) syind sorted_yind).
+    rewrite -yindE...
+    suff: (y <= yind[iy]) by lia.
+    rewrite yindE; first apply/In_lt; rewrite ?sE -?yindE... }
+  { move=> l *; rewrite /Inv/op/ntriple.
+    xpull=> ix iy []_[]?[]?[]L1[]L2; rewrite /cond; bool_rew=> /[!not_and_eq]-[] []G _.
+    { rewrite /R1.
+      xin (3,0): fold'; xapp get_spec=> *...
+      rewrite /R2.
+      xapp get_spec_out_unary...
+      { move/max_le; move: L1; rewrite take_ge ?length_List_length; try math.
+        rewrite -/(slice _ _ _)-/sxind; lia. }
+      xsimpl; try math.
+      splits*=> //.
+      { move=> ?. suff: ind[l] < ind[l+1] by lia.
+        apply/sorted_le; autos*; try lia.
+        exact/sorted_merge. }
+      { move=> ?. suff: ind[l] < ind[l+1] by lia.
+        apply/sorted_le; autos*; try lia.
+        exact/sorted_merge. }
+        bool_rew; lia. }
+    rewrite /R2.
+    xin (2,0): fold'; xapp get_spec=> *...
+    rewrite /R1.
+    xapp get_spec_out_unary...
+    { move/max_le; move: L2; rewrite take_ge ?length_List_length; try math.
+      rewrite -/(slice _ _ _)-/syind; lia. }
+    xsimpl; try lia.
+    splits*=> //.
+    { move=> ?. suff: ind[l] < ind[l+1] by lia.
+      apply/sorted_le; autos*; try lia.
+      exact/sorted_merge. }
+    { move=> ?. suff: ind[l] < ind[l+1] by lia.
+      apply/sorted_le; autos*; try lia.
+      exact/sorted_merge. }
+    bool_rew; lia. }
+  { move=> ???. rewrite /ntriple -xnwp1_lemma /=.
+    rewrite /Inv; xpull=> ix iy C.
+    do ? (xwp; xapp). xapp @and.spec=> //.
+    move=> ? E'; bool_rew; case: (C)=> ? [?][?][?][?][] ?.
+    xsimpl=> // ?; subst; rewrite E' /cond. by bool_rew.  }
+  { move=> ?? []/(_ eq_refl); by case: b. }
+  { move=> *. move/NoDup_nthZ: ndind=> /[apply]; lia. }
+  { move=> *. move/NoDup_nthZ: ndind=> /[apply]; lia. }
+  { rewrite /arr1 /Inv/arrs/arr1; xsimpl lbx lby.
+    { splits; [|lia|lia| | |autos*|].
+      { rewrite /cond/ind; bool_rew; move: (size_merge sxind syind); lia. }
+        { rewrite Z.sub_diag abs_0 /= max0=> ?.
+          have: (In (nth 0 ind 0) ind) by apply/nth_In; lia.
+          rewrite In_merge=> -[/xind_leq|/yind_leq]; lia. }
+        { rewrite Z.sub_diag abs_0 /= max0=> ?.
+          have: (In (nth 0 ind 0) ind) by apply/nth_In; lia.
+          rewrite In_merge=> -[/xind_leq|/yind_leq]; lia. }
+        rewrite /cond; bool_rew; do ? split; rewrite ?xindE ?yindE ?Z.sub_diag...
+        { rewrite merge_nth0... }
+        { move=> ?/(In_le_0 _ _ sorted_xind); rewrite -/sxind; lia. }
+        move=> ?/(In_le_0 _ _ sorted_yind); rewrite -/syind; lia. }
+    rewrite /H2/H1 ?E (fset_of_list_nodup 0) // /R1 /R2.
+    rewrite -> ?hbig_fset_hstar; xsimpl*. }
+  simpl=> v; rewrite /op/R1/R2/Inv/arr1/arrs/H2/H1 E -fset_of_list_nodup //.
+  rewrite -> ?hbig_fset_hstar; xsimpl=> ?? _. 
+  do 4 (xwp; xapp); xwp; xval; xsimpl; rewrite /op.
+  rewrite (@SumEq _ _
+    (fun i => If ind i then v[`2](i) *  v[`3](i) else 0) 
+    `[0, M]).
+  { rewrite (SumIf (fun=> id)) E (SumList 0) // Sum0s; f_equal; math. }
+  by move=> ?; case: classicT.
+Qed.
+
+End sv.
+*)
+End sv.
